day 1

Aoc2023/Utils.lean
@@ -1,11 +1,26 @@
 import Lean.Data.Parsec
+import Std.Data.Nat.Lemmas
+import Std.Data.Array.Lemmas
+import Init.Data.String.Basic
+import Aoc2023.AesopExtra
+
+namespace Char
+
+def toNatDigit (c : Char) : Nat :=
+  c.toNat - 48
+
+end Char
 
 namespace Array
 
 def max [Inhabited α] [Max α] (a : Array α) : α :=
-  if a.size = 0 then default else Array.foldl Max.max a[0]! a
+  if h : a.size = 0 then
+    default
+  else
+    have : 0 < a.size := Nat.pos_of_ne_zero h
+    a.foldl (init := a[0]) Max.max
 
-def findIdx! (as : Array α) (p : α → Bool) : Nat := 
+def findIdx! (as : Array α) (p : α → Bool) : Nat :=
   match as.findIdx? p with
   | some x => x
   | none => panic!"Element not found"
@@ -18,7 +33,7 @@ def filterWithIdx (as : Array α) (p : Nat → α → Bool) : Array α :=
       (idx+1, r)
 
 def mkArray₂ (m n : Nat) (v : α) : Array (Array α) :=
-  Array.mkArray m (Array.mkArray n v) 
+  Array.mkArray m (Array.mkArray n v)
 
 def foldtlM [Monad m] (f : β → α → m β) (init : β) (a : Array (Array α)) : m β :=
   a.foldlM (fun x row => row.foldlM f x) init
@@ -40,9 +55,25 @@ def zipWith2D (a : Array (Array α)) (b : Array (Array β)) (f : α → β → �
 def modify₂ (a : Array (Array α)) (i j : Nat) (f : α → α) : Array (Array α) :=
   a.modify i (·.modify j f)
 
-def sum [Add α] (a : Array α) : Option α := a.foldl (fun s elem => match s with
-                                                                   | none => some elem
-                                                                   | some x => some (x + elem)) none 
+def set₂ (a : Array (Array α)) (i j : Nat) (x : α) : Array (Array α) :=
+  a.modify i (·.modify j (fun _ => x))
+
+def sum [Add α] [OfNat α 0] (a : Array α) : α := a.foldl (init := 0) (· + ·)
+
+def containsAny (as : Array α) (p : α → Bool) : Bool := Id.run do
+  for a in as do
+    if p a then return true
+  return false
+
+def Pairwise (as : Array α) (r : α → α → Prop) :=
+  ∀ i j : Nat, (hi : i < as.size) → (hj : j < as.size) → i ≠ j → r as[i] as[j]
+
+def Nodup [DecidableEq α] (as : Array α) : Prop :=
+  as.Pairwise (· ≠ ·)
+
+-- FOR STD
+
+theorem size_empty : (#[] : Array α).size = 0 := List.length_nil
 
 end Array
 
@@ -52,12 +83,94 @@ def toCharArray (s : String) : Array Char := s.data.toArray
 
 def ofCharArray (a : Array Char) : String := { data := a.toList }
 
-def yoloParse [Inhabited α] (s : String) (p : Lean.Parsec α) : α := 
+def reverse (s : String) : String :=
+  s.foldr (init := "") fun c t => t.push c
+
+def yoloParse [Inhabited α] (s : String) (p : Lean.Parsec α) : α :=
   match p s.iter with
-  | Lean.Parsec.ParseResult.success _ x => x 
+  | Lean.Parsec.ParseResult.success _ x => x
   | Lean.Parsec.ParseResult.error _ _ => panic! "YOLO!"
 
+def parse? [Inhabited α] (s : String) (p : Lean.Parsec α) : Option α :=
+  match p s.iter with
+  | Lean.Parsec.ParseResult.success _ x => some x
+  | Lean.Parsec.ParseResult.error _ _ => none
+
 end String
+
+/-- Simple set structure where we just put elements into an array. -/
+structure ArraySet (α : Type _) [DecidableEq α] where
+  content : Array α
+  nodup : content.Nodup
+
+namespace ArraySet
+
+variable [DecidableEq α]
+
+--def Any (p : α → Prop) (as : ArraySet α) : Prop :=
+--  ∃ i, (h : i < as.content.size) → p as.content[i]
+
+instance : Membership α (ArraySet α) where
+  mem x as := x ∈ as.content
+
+theorem mem_def (as : ArraySet α) (x : α) : x ∈ as ↔ x ∈ as.content := Iff.rfl
+
+instance instDecidableMem {x : α} {as : ArraySet α} : Decidable (x ∈ as) :=
+  inferInstanceAs (Decidable (x ∈ as.content))
+
+--instance instDecidableMem {as : ArraySet α} : Decidable (Mem x as) :=
+
+def mkEmpty : ArraySet α where
+  content := #[]
+  nodup := fun _ _ hi _ _ => by simp [Array.size_empty, Nat.not_lt_zero] at hi
+
+def contains (as : ArraySet α) (x : α) : Bool := as.content.contains x
+
+def card (as : ArraySet α) : Nat := as.content.size
+
+theorem contains_iff (as : ArraySet α) (x : α) :
+    as.contains x = true ↔ x ∈ as := by rw [contains]; exact Array.contains_def
+
+theorem not_eq_getElem_of_not_mem (as : ArraySet α) {x : α} (hx : x ∉ as) :
+    ∀ i, (h : i < as.content.size) → as.content[i] ≠ x := by
+  intro i hi
+  rw [mem_def, Array.mem_def, List.mem_iff_get, not_exists] at hx
+  specialize hx ⟨i, hi⟩
+  rwa [Array.getElem_eq_data_get]
+
+theorem exists_getElem_of_mem (as : ArraySet α) {x : α} (hx : x ∈ as) :
+    ∃ (i : Fin as.content.size), as.content[i] = x := by
+  rw [mem_def, Array.mem_def, List.mem_iff_get] at hx
+  obtain ⟨i, hi⟩ := hx
+  refine ⟨i, ?_⟩
+  rwa [← Array.getElem_eq_data_get] at hi
+
+def insert (as : ArraySet α) (x : α) : ArraySet α :=
+  if hmem : x ∈ as then
+    as
+  else
+    { content := as.content.push x,
+      nodup := by
+        unfold Array.Nodup Array.Pairwise
+        intro i j hi hj hij
+        simp only [Array.get_push]
+        split
+        case inl h =>
+          split
+          case inl h₂ => exact as.nodup i j h h₂ hij
+          case inr h₂ =>
+            have := not_eq_getElem_of_not_mem as hmem
+            exact fun hmain => False.elim <| (this i h) hmain
+        case inr h =>
+          split
+          case inl h₂ =>
+            have := not_eq_getElem_of_not_mem as hmem
+            exact fun hmain => False.elim <| (this j h₂) hmain.symm
+          case inr h₂ =>
+            rw [Array.size_push, ←Nat.succ_eq_add_one, Nat.lt_succ] at hi hj
+            aesop }
+
+end ArraySet
 
 namespace Lean.Parsec
 
@@ -65,13 +178,15 @@ def natNum : Parsec Nat := do
   let some n := (← manyChars digit).toNat? | fail "Not a natural number"
   return n
 
+def natDigit : Parsec Nat := return (← digit).toNatDigit
+
 def newlineChar : Parsec Unit := attempt do
   let c ← anyChar
   if c == '\u000a' || c == '\u000a' then return () else fail s!"Newline not found"
 
 def eol : Parsec Unit := eof <|> (many1 newlineChar *> pure ())
 
-partial def sepByCore (pcont : Parsec α) (psep : Parsec β) (acc : List α) : 
+partial def sepByCore (pcont : Parsec α) (psep : Parsec β) (acc : List α) :
   Parsec (List α) :=
 (do let _ ← psep; sepByCore pcont psep (acc ++ [←pcont])) <|> pure acc
 
