Aoc2023.lean
@@ -1,3 +1,4 @@
 -- This module serves as the root of the `Aoc2023` library.
 -- Import modules here that should be built as part of the library.
-import «Aoc2023».Basic
+import Aoc2023.Utils
+--import Aoc2023.Scratchpad
