Aoc2023/Day01.lean
@@ -5,6 +5,7 @@ open System
 namespace Day01
 
 def testinput : FilePath := "/home/fred/lean/aoc2023/input_01_test"
+def testinput2 : FilePath := "/home/fred/lean/aoc2023/input_01_test2"
 def realinput : FilePath := "/home/fred/lean/aoc2023/input_01"
 
 /-
@@ -12,9 +13,10 @@ PART 1:
 -/
 
 def first_part (input : FilePath) : IO Nat := do
-  IO.println ""
   let rawdata := (← IO.FS.lines input)
-  return 0
+  let data := rawdata.map (fun s => s.toCharArray.filter (·.isDigit))
+                    |>.map fun as => as[0]!.toNatDigit * 10 + as[as.size-1]!.toNatDigit
+  return data.sum
 
 --#eval first_part testinput
 --#eval first_part realinput
@@ -23,11 +25,48 @@ def first_part (input : FilePath) : IO Nat := do
 PART 2:
 -/
 
+open Lean Lean.Parsec
+
+def parseNumberForwards : Parsec Nat :=
+  natDigit
+  <|> (do let _ ← pstring "zero"; return 0)
+  <|> (do let _ ← pstring "one"; return 1)
+  <|> (do let _ ← pstring "two"; return 2)
+  <|> (do let _ ← pstring "three"; return 3)
+  <|> (do let _ ← pstring "four"; return 4)
+  <|> (do let _ ← pstring "five"; return 5)
+  <|> (do let _ ← pstring "six"; return 6)
+  <|> (do let _ ← pstring "seven"; return 7)
+  <|> (do let _ ← pstring "eight"; return 8)
+  <|> (do let _ ← pstring "nine"; return 9)
+
+def parseNumberBackwards : Parsec Nat :=
+  natDigit
+  <|> (do let _ ← pstring "zero".reverse; return 0)
+  <|> (do let _ ← pstring "one".reverse; return 1)
+  <|> (do let _ ← pstring "two".reverse; return 2)
+  <|> (do let _ ← pstring "three".reverse; return 3)
+  <|> (do let _ ← pstring "four".reverse; return 4)
+  <|> (do let _ ← pstring "five".reverse; return 5)
+  <|> (do let _ ← pstring "six".reverse; return 6)
+  <|> (do let _ ← pstring "seven".reverse; return 7)
+  <|> (do let _ ← pstring "eight".reverse; return 8)
+  <|> (do let _ ← pstring "nine".reverse; return 9)
+
+partial def getFirstNum : Parsec Nat :=
+  parseNumberForwards <|> (do let _ ← anyChar; getFirstNum)
+
+partial def getFirstNumBackwards : Parsec Nat :=
+  parseNumberBackwards <|> (do let _ ← anyChar; getFirstNumBackwards)
+
 def second_part (input : FilePath) : IO Nat := do
   let rawdata := (← IO.FS.lines input)
-  return 0
+  let firstDigits := rawdata.map fun s => s.yoloParse getFirstNum
+  let lastDigits := rawdata.map fun s => s.reverse.yoloParse getFirstNumBackwards
+  let lines := firstDigits.zipWith lastDigits fun a b => 10*a + b
+  return lines.sum
 
---#eval second_part testinput
+--#eval second_part testinput2
 --#eval second_part realinput
 
 end Day01
