Aoc2023/Scratchpad.lean
@@ -1,4 +1,7 @@
 import Aoc2023.Utils
+import Std.Data.RBMap.Basic
+
+open Std
 
 --def produitChaine (r c : Array Nat) : Array (Array Nat) := Id.run do
 --  --if rows.size ≠ cols.size then panic!
@@ -14,6 +17,66 @@ import Aoc2023.Utils
 --  return m
 --
 --#eval produitChaine #[0, 10, 30, 5, 60, 3] #[0, 30, 5, 60, 3, 8]
+
+inductive Lettre
+| a
+| b
+| c
+deriving BEq, Repr
+
+instance : ToString Lettre where
+  toString x := match x with
+                | .a => "a"
+                | .b => "b"
+                | .c => "c"
+
+instance : Mul Lettre where
+  mul x y := match x, y with
+             | .a, .a => .c
+             | .a, .b => .c
+             | .a, .c => .a
+             | .b, .a => .c
+             | .b, .b => .b
+             | .b, .c => .a
+             | .c, .a => .a
+             | .c, .b => .c
+             | .c, .c => .c
+
+def Lettre.cmp : Lettre → Lettre → Ordering
+| .a, .a => .eq
+| .a, .b => .lt
+| .a, .c => .lt
+| .b, .a => .gt
+| .b, .b => .eq
+| .b, .c => .lt
+| .c, .a => .gt
+| .c, .b => .gt
+| .c, .c => .eq
+
+def mulSets (xs ys : RBSet Lettre Lettre.cmp) : RBSet Lettre Lettre.cmp := Id.run do
+  let mut out := mkRBSet Lettre Lettre.cmp
+  for x in xs do
+    for y in ys do
+      if ¬out.contains (x*y) then
+        out := out.insert <| x * y
+  return out
+
+def fillTable (input : Array Lettre) : Array (Array (Array Lettre)) := Id.run do
+  let n := input.size
+  let mut table : Array (Array (Array Lettre)) := #[input.map fun x => #[x]]
+  for len in [2:n+1] do
+    let mut curRow : Array (Array Lettre) := #[]
+    for startPos in [0:n-len] do
+      let mut curPos : Array Lettre := #[]
+      for pos in [0:len-1] do
+        curPos := curPos.push <| mulSets table[pos]![startPos]! table[len-(pos+1)-1]![startPos+pos+1]!
+        dbg_trace s!"len = {len}, startPos = {startPos}, curPos = {curPos}"
+      curRow := curRow.push curPos
+    table := table.push curRow
+  return table
+
+#eval mulSets #[.b] #[.a, .b]
+#eval fillTable #[.b, .b, .b, .b, .a]
 
 structure Dummy where
   func : Nat → Nat
