Main.lean
@@ -1,11 +1,11 @@
-import Aoc2023
+import Aoc2023.Day01
 
 def main (args : List String) : IO Unit :=
   match args with
   | ["1"] => do
     IO.println "Day 1:"
-    IO.println s!"Part 1: {← Day1.first_part}"
-    IO.println s!"Part 2: {← Day1.second_part}"
+    IO.println s!"Part 1: {← Day01.first_part "input_01"}"
+    IO.println s!"Part 2: {← Day01.second_part "input_01"}"
     IO.println ""
   | _ => do
     IO.println "Help, what should I do!?"
